WIP: update Compatibility.v

src/trans/Compatibility.v
@@ -52,13 +52,13 @@ Definition _sim_itree
            R_src R_tgt
            (sim_ret:SIM_VAL R_src R_tgt)
            (itr_src: itree MemE.t R_src) (itr_tgt: itree MemE.t R_tgt): Prop :=
-  forall lc_src lc_tgt sc0_src sc0_tgt mem0_src mem0_tgt
+  forall lc_src lc_tgt gl0_src gl0_tgt
     (LOCAL: sim_local lc_src lc_tgt),
     sim_thread
       (lang R_src) (lang R_tgt)
       (sim_terminal sim_ret)
-      itr_src lc_src sc0_src mem0_src
-      itr_tgt lc_tgt sc0_tgt mem0_tgt.
+      itr_src lc_src gl0_src
+      itr_tgt lc_tgt gl0_tgt.
 
 Definition _sim_ktree
            (sim_thread:SIM_THREAD)
@@ -72,14 +72,14 @@ Definition _sim_ktree
     _sim_itree sim_thread sim_ret1 (ktr_src r_src) (ktr_tgt r_tgt).
 
 Lemma _sim_itree_mon
-      s1 s2 (S: s1 <11= s2):
+      s1 s2 (S: s1 <9= s2):
   @_sim_itree s1 <5= @_sim_itree s2.
 Proof.
   ii. apply S. apply PR; auto.
 Qed.
 
 Lemma _sim_ktree_mon
-      s1 s2 (S: s1 <11= s2):
+      s1 s2 (S: s1 <9= s2):
   @_sim_ktree s1 <8= @_sim_ktree s2.
 Proof.
   ii. apply S. apply PR; auto.
@@ -97,19 +97,20 @@ Proof.
 Qed.
 
 Lemma program_step_bind R0 R1
-      (itr0 itr1: itree MemE.t R0) (k: R0 -> itree MemE.t R1) e
-      lc1 sc1 mem1
-      lc2 sc2 mem2
-      (STEP: Thread.program_step
-               e
-               (Thread.mk (lang R0) itr0 lc1 sc1 mem1)
-               (Thread.mk (lang R0) itr1 lc2 sc2 mem2)):
-  Thread.program_step
-    e
-    (Thread.mk (lang R1) (itr0 >>= k) lc1 sc1 mem1)
-    (Thread.mk (lang R1) (itr1 >>= k) lc2 sc2 mem2).
+      (itr0 itr1: itree MemE.t R0) (k: R0 -> itree MemE.t R1)
+      reserved e
+      lc1 gl1
+      lc2 gl2
+      (STEP: Thread.step
+               reserved true e
+               (Thread.mk (lang R0) itr0 lc1 gl1)
+               (Thread.mk (lang R0) itr1 lc2 gl2)):
+  Thread.step
+    reserved true e
+    (Thread.mk (lang R1) (itr0 >>= k) lc1 gl1)
+    (Thread.mk (lang R1) (itr1 >>= k) lc2 gl2).
 Proof.
-  inv STEP; inv LOCAL; ss.
+  inv STEP. inv LOCAL; ss.
   - econs; [|econs 1]; s; eauto. apply lang_step_bind. auto.
   - econs; [|econs 2]; s; eauto. apply lang_step_bind. auto.
   - econs; [|econs 3]; s; eauto. apply lang_step_bind. auto.
@@ -120,35 +121,36 @@ Proof.
   - econs; [|econs 8]; s; eauto. apply lang_step_bind. auto.
   - econs; [|econs 9]; s; eauto. apply lang_step_bind. auto.
   - econs; [|econs 10]; s; eauto. apply lang_step_bind. auto.
-  - econs; [|econs 11]; s; eauto. apply lang_step_bind. auto.
 Qed.
 
 Lemma step_bind R0 R1
-      (itr0 itr1: itree MemE.t R0) (k: R0 -> itree MemE.t R1) pf e
-      lc1 sc1 mem1
-      lc2 sc2 mem2
-      (STEP: Thread.step pf e
-                         (Thread.mk (lang R0) itr0 lc1 sc1 mem1)
-                         (Thread.mk (lang R0) itr1 lc2 sc2 mem2)):
-  Thread.step pf e
-              (Thread.mk (lang R1) (itr0 >>= k) lc1 sc1 mem1)
-              (Thread.mk (lang R1) (itr1 >>= k) lc2 sc2 mem2).
+      (itr0 itr1: itree MemE.t R0) (k: R0 -> itree MemE.t R1)
+      reserved pf e
+      lc1 gl1
+      lc2 gl2
+      (STEP: Thread.step reserved pf e
+                         (Thread.mk (lang R0) itr0 lc1 gl1)
+                         (Thread.mk (lang R0) itr1 lc2 gl2)):
+  Thread.step reserved pf e
+              (Thread.mk (lang R1) (itr0 >>= k) lc1 gl1)
+              (Thread.mk (lang R1) (itr1 >>= k) lc2 gl2).
 Proof.
   inv STEP.
-  - econs 1. inv STEP0. econs; eauto.
-  - econs 2. apply program_step_bind. eauto.
+  - econs 1. inv LOCAL; econs; eauto.
+  - apply program_step_bind. eauto.
 Qed.
 
 Lemma opt_step_bind R0 R1
-      (itr0 itr1: itree MemE.t R0) (k: R0 -> itree MemE.t R1) e
-      lc1 sc1 mem1
-      lc2 sc2 mem2
-      (STEP: Thread.opt_step e
-                             (Thread.mk (lang R0) itr0 lc1 sc1 mem1)
-                             (Thread.mk (lang R0) itr1 lc2 sc2 mem2)):
-  Thread.opt_step e
-                  (Thread.mk (lang R1) (itr0 >>= k) lc1 sc1 mem1)
-                  (Thread.mk (lang R1) (itr1 >>= k) lc2 sc2 mem2).
+      (itr0 itr1: itree MemE.t R0) (k: R0 -> itree MemE.t R1)
+      reserved pf e
+      lc1 gl1
+      lc2 gl2
+      (STEP: Thread.opt_step reserved pf e
+                             (Thread.mk (lang R0) itr0 lc1 gl1)
+                             (Thread.mk (lang R0) itr1 lc2 gl2)):
+  Thread.opt_step reserved pf e
+                  (Thread.mk (lang R1) (itr0 >>= k) lc1 gl1)
+                  (Thread.mk (lang R1) (itr1 >>= k) lc2 gl2).
 Proof.
   inv STEP.
   - econs 1.
@@ -157,33 +159,34 @@ Qed.
 
 Lemma thread_step_deseq
       R0 R1 ktr (itr1: itree MemE.t R0) (itr2: itree MemE.t R1)
-      pf e
-      lc1 sc1 mem1
-      lc2 sc2 mem2
-      (STEP: Thread.step pf e
-                         (Thread.mk (lang _) (itr1 >>= ktr) lc1 sc1 mem1)
-                         (Thread.mk (lang _) itr2 lc2 sc2 mem2)):
+      reserved pf e
+      lc1 gl1
+      lc2 gl2
+      (STEP: Thread.step reserved pf e
+                         (Thread.mk (lang _) (itr1 >>= ktr) lc1 gl1)
+                         (Thread.mk (lang _) itr2 lc2 gl2)):
   (exists r,
       itr1 = Ret r /\
-      Thread.step pf e
-                  (Thread.mk (lang _) (ktr r) lc1 sc1 mem1)
-                  (Thread.mk (lang _) (itr2) lc2 sc2 mem2)) \/
+      Thread.step reserved pf e
+                  (Thread.mk (lang _) (ktr r) lc1 gl1)
+                  (Thread.mk (lang _) (itr2) lc2 gl2)) \/
   (exists itr2',
       itr2 = itr2' >>= ktr /\
-      Thread.step pf e
-                  (Thread.mk (lang _) itr1 lc1 sc1 mem1)
-                  (Thread.mk (lang _) itr2' lc2 sc2 mem2)) \/
+      Thread.step reserved pf e
+                  (Thread.mk (lang _) itr1 lc1 gl1)
+                  (Thread.mk (lang _) itr2' lc2 gl2)) \/
   (itr1 = Vis MemE.abort (Empty_set_rect _) /\
    e = ThreadEvent.failure)
 .
 Proof.
   inv STEP.
-  - inv STEP0. right. left. esplits; eauto.
-    econs 1. econs; eauto.
-  - inv STEP0; ss.
-    apply lang_step_deseq in STATE. des; clarify.
-    { left. esplits; eauto. econs 2. econs; eauto. }
-    { right. left. esplits; eauto. econs 2. econs; eauto. }
+  - inv LOCAL.
+    + right. left. esplits; eauto. econs 1. econs 1. eauto.
+    + right. left. esplits; eauto. econs 1. econs 2. eauto.
+    + right. left. esplits; eauto. econs 1. econs 3. eauto.
+  - apply lang_step_deseq in STATE. des; clarify.
+    { left. esplits; eauto. }
+    { right. left. esplits; eauto. }
     { destruct e; ss; auto. }
 Qed.
 
@@ -210,22 +213,23 @@ Qed.
 Inductive sim_bind R0 R1 (k: R0 -> itree MemE.t R1):
   forall (lhs: Thread.t (lang R0)) (rhs:Thread.t (lang R1)), Prop :=
 | sim_bind_intro
-    itr lc sc mem:
+    itr lc gl:
     sim_bind k
-             (Thread.mk (lang R0) itr lc sc mem)
-             (Thread.mk (lang R1) (itr >>= k) lc sc mem)
+             (Thread.mk (lang R0) itr lc gl)
+             (Thread.mk (lang R1) (itr >>= k) lc gl)
 .
 
 Lemma rtc_internal_step_bind R0 R1
       (itr0 itr1: itree MemE.t R0) (k: R0 -> itree MemE.t R1)
-      lc1 sc1 mem1
-      lc2 sc2 mem2
-      (STEP: rtc (@Thread.tau_step (lang R0))
-                 (Thread.mk (lang R0) itr0 lc1 sc1 mem1)
-                 (Thread.mk (lang R0) itr1 lc2 sc2 mem2)):
-  rtc (@Thread.tau_step (lang R1))
-      (Thread.mk (lang R1) (itr0 >>= k) lc1 sc1 mem1)
-      (Thread.mk (lang R1) (itr1 >>= k) lc2 sc2 mem2).
+      reserved
+      lc1 gl1
+      lc2 gl2
+      (STEP: rtc (@Thread.tau_step (lang R0) reserved)
+                 (Thread.mk (lang R0) itr0 lc1 gl1)
+                 (Thread.mk (lang R0) itr1 lc2 gl2)):
+  rtc (@Thread.tau_step (lang R1) reserved)
+      (Thread.mk (lang R1) (itr0 >>= k) lc1 gl1)
+      (Thread.mk (lang R1) (itr1 >>= k) lc2 gl2).
 Proof.
   exploit (sim_rtc (sim_bind k)); eauto.
   - i. inv SIM1. destruct a2. destruct local. inv RA. inv TSTEP.
@@ -237,57 +241,57 @@ Proof.
 Qed.
 
 
-Global Hint Resolve cpn11_wcompat: paco.
+Global Hint Resolve cpn9_wcompat: paco.
 
 Inductive ctx (sim_thread:SIM_THREAD): SIM_THREAD :=
 | ctx_ret
     R_src R_tgt
     (sim_ret:SIM_VAL R_src R_tgt)
-    sc0_src mem0_src
-    sc0_tgt mem0_tgt
+    gl0_src
+    gl0_tgt
     lc_src lc_tgt (r_src: R_src) (r_tgt: R_tgt)
     (RET: sim_ret r_src r_tgt)
-    (LOCAL: sim_local SimPromises.bot lc_src lc_tgt):
+    (LOCAL: sim_local lc_src lc_tgt):
     @ctx sim_thread
          (lang R_src) (lang R_tgt)
          (sim_terminal sim_ret)
-         (Ret r_src) lc_src sc0_src mem0_src
-         (Ret r_tgt) lc_tgt sc0_tgt mem0_tgt
+         (Ret r_src) lc_src gl0_src
+         (Ret r_tgt) lc_tgt gl0_tgt
 | ctx_bind
     R_src0 R_tgt0 R_src1 R_tgt1
     (sim_ret1:SIM_VAL R_src0 R_tgt0) (sim_ret2:SIM_VAL R_src1 R_tgt1)
-    itr0 k0 lc_src sc0_src mem0_src
-    itr1 k1 lc_tgt sc0_tgt mem0_tgt
+    itr0 k0 lc_src gl0_src
+    itr1 k1 lc_tgt gl0_tgt
     (SIM1: sim_thread (lang R_src0) (lang R_tgt0) (sim_terminal sim_ret1)
-                      itr0 lc_src sc0_src mem0_src
-                      itr1 lc_tgt sc0_tgt mem0_tgt)
+                      itr0 lc_src gl0_src
+                      itr1 lc_tgt gl0_tgt)
     (SIM2: _sim_ktree sim_thread sim_ret1 k0 k1 sim_ret2):
     @ctx sim_thread
          (lang R_src1) (lang R_tgt1)
          (sim_terminal sim_ret2)
-         (itr0 >>= k0) lc_src sc0_src mem0_src
-         (itr1 >>= k1) lc_tgt sc0_tgt mem0_tgt
+         (itr0 >>= k0) lc_src gl0_src
+         (itr1 >>= k1) lc_tgt gl0_tgt
 | ctx_tau_iter
     I_src I_tgt R_src R_tgt
     (sim_ret0: SIM_VAL I_src I_tgt) (sim_ret1: SIM_VAL R_src R_tgt)
-    sc0_src mem0_src
-    sc0_tgt mem0_tgt
+    gl0_src
+    gl0_tgt
     lc_src lc_tgt
     (body_src: I_src -> itree MemE.t (I_src + R_src))
     (body_tgt: I_tgt -> itree MemE.t (I_tgt + R_tgt))
     (SIM: _sim_ktree sim_thread sim_ret0 body_src body_tgt (sum_rel sim_ret0 sim_ret1))
     i_src i_tgt
     (VAL: sim_ret0 i_src i_tgt)
-    (LOCAL: sim_local SimPromises.bot lc_src lc_tgt)
+    (LOCAL: sim_local lc_src lc_tgt)
   :
     @ctx sim_thread
               (lang R_src) (lang R_tgt)
               (sim_terminal sim_ret1)
-              (tau;;(ITree.iter body_src i_src)) lc_src sc0_src mem0_src
-              (tau;;(ITree.iter body_tgt i_tgt)) lc_tgt sc0_tgt mem0_tgt
+              (tau;;(ITree.iter body_src i_src)) lc_src gl0_src
+              (tau;;(ITree.iter body_tgt i_tgt)) lc_tgt gl0_tgt
 .
 
-Lemma ctx_mon: monotone11 ctx.
+Lemma ctx_mon: monotone9 ctx.
 Proof.
   ii. destruct IN.
   - econs 1; eauto.
@@ -298,205 +302,205 @@ Qed.
 
 
 Lemma ctx_compat:
-  ctx <12= gupaco11 _sim_thread (cpn11 _sim_thread).
+  ctx <10= gupaco9 _sim_thread (cpn9 _sim_thread).
 Proof.
-  assert (MON: monotone11 _sim_thread).
-  (* paco tactics do not work well without this *)
-  { eapply _sim_thread_mon; eauto. }
-  eapply wrespect11_uclo; auto.
-  econs; auto with paco. i. destruct PR.
-  - (* ret *)
-    ii.
-    inversion LOCAL. apply SimPromises.sem_bot_inv in PROMISES; auto.
-    destruct lc_src, lc_tgt. ss. subst.
-    splits; s; ii.
-    { right. inv TERMINAL_TGT. ss. esplits; eauto; ss.
-      - econs; eauto.
-      - econs; eauto.
-    }
-    { right. subst. esplits; eauto. }
-    inv STEP_TGT; try by inv STEP; inv STATE.
-    inv STEP; ss.
-    exploit sim_local_promise; eauto. i. des.
-    right. esplits.
-    + ss.
-    + eauto.
-    + econs 2. econs 1. econs; eauto.
-    + eauto.
-    + eauto.
-    + eauto.
-    + eapply rclo11_clo_base. eapply ctx_ret; auto.
-  - (* bind *)
-    ii. ss. eapply GF in SIM1.
-    exploit SIM1; try apply SC; eauto. i. des.
-    splits; s; ii.
-    { inv TERMINAL_TGT. ides itr1.
-      2: { eapply f_equal with (f:=observe) in H. ss. }
-      2: { eapply f_equal with (f:=observe) in H. ss. }
-      rewrite bind_ret_l in H.
-      exploit TERMINAL; try by econs. i. des.
-      - left.
-        unfold Thread.steps_failure in *. des.
-        destruct e2, e3.
-        eapply rtc_internal_step_bind in STEPS.
-        eapply step_bind in STEP_FAILURE.
-        esplits; eauto.
-      - inversion LOCAL. exploit SimPromises.sem_bot_inv; eauto. i.
-        destruct lc2_src. ss. subst.
-        inv TERMINAL_SRC.
-        exploit Thread.rtc_tau_step_future; eauto. s. i. des.
-        inv TERMINAL0. ss.
-        assert (x0 = r1).
-        { eapply f_equal with (f:=observe) in SRC. ss. clarify. }
-        assert (r0 = r2).
-        { eapply f_equal with (f:=observe) in TGT. ss. clarify. }
-        subst.
-        exploit SIM2; eauto. intros x0. eapply GF in x0.
-        exploit x0; try apply SC0; eauto using Memory.future_future_weak.
-        i. ss. des. exploit TERMINAL0; try by econs.
-        { econs. eauto. }
-        i. des.
-        + left.
-          unfold Thread.steps_failure in *. des.
-          destruct e2.
-          esplits; [|eauto|eauto].
-          etrans; try exact STEPS0.
-          eapply rtc_internal_step_bind in STEPS.
-          rewrite bind_ret_l in STEPS. eauto.
-        + right.
-          destruct lc2_src.
-          esplits; cycle 1; eauto.
-          * rewrite bind_ret_l. eauto.
-          * etrans; [|eauto].
-            eapply rtc_internal_step_bind in STEPS.
-            rewrite bind_ret_l in STEPS. eauto.
-    }
-    { exploit PROMISES; eauto. i. des.
-      - left.
-        unfold Thread.steps_failure in *. des.
-        destruct e2, e3.
-        eapply rtc_internal_step_bind in STEPS.
-        eapply step_bind in STEP_FAILURE.
-        esplits; eauto.
-      - right.
-        destruct lc_tgt, lc2_src. ss. subst.
-        esplits; [|eauto].
-        + eapply rtc_internal_step_bind. apply STEPS.
-        + ss.
-    }
-    hexploit thread_step_deseq; eauto. i. des; clarify.
-    + exploit TERMINAL; try by econs. i. des.
-      * left.
-        unfold Thread.steps_failure in *. des.
-        destruct e2, e3. ss.
-        eapply rtc_internal_step_bind in STEPS.
-        eapply step_bind in STEP_FAILURE.
-        esplits; eauto.
-      * inversion LOCAL. exploit SimPromises.sem_bot_inv; eauto. i. subst.
-        destruct lc2_src. inv TERMINAL_SRC. ss. subst.
-        exploit Thread.rtc_tau_step_future; eauto. s. i. des.
-        inv TERMINAL0. ss. subst.
-        assert (x = r1).
-        { eapply f_equal with (f:=observe) in SRC. ss. clarify. }
-        assert (r0 = r2).
-        { eapply f_equal with (f:=observe) in TGT. ss. clarify. }
-        subst.
-        exploit SIM2; eauto. intros x. eapply GF in x.
-        exploit x; try apply SC0; eauto using Memory.future_future_weak.
-        i. ss. des.
-        exploit STEP0; eauto. i. des.
-        { left.
-          unfold Thread.steps_failure in *. des.
-          destruct e2, e3.
-          eapply rtc_internal_step_bind in STEPS.
-          esplits; try exact STEP_FAILURE; [|eauto].
-          etrans; eauto. rewrite bind_ret_l. eauto. }
-        { right.
-          esplits; cycle 2; eauto.
-          - eapply rclo11_base. auto.
-          - eapply rtc_internal_step_bind in STEPS.
-            etrans; [apply STEPS|eauto].
-            rewrite bind_ret_l. eauto. }
-    + destruct lc3_tgt.
-      exploit STEP; eauto. i. des.
-      * left.
-        unfold Thread.steps_failure in *. des.
-        destruct e2, e3.
-        eapply rtc_internal_step_bind in STEPS.
-        eapply step_bind in STEP_FAILURE.
-        esplits; eauto.
-      * right.
-        destruct lc2_src. destruct lc3_src.
-        esplits; [|M|M| | | |]; Mskip eauto.
-        { eapply rtc_internal_step_bind. eauto. }
-        { eapply opt_step_bind. eauto. }
-        { eapply rclo11_clo_base. eapply ctx_bind; eauto.
-          eapply _sim_ktree_mon; cycle 1; eauto.
-        }
-    + left. exploit STEP.
-      { right. instantiate (5:=ThreadEvent.failure). econs; eauto.
-        ss. econs; eauto. }
-      i. des; ss.
-      unfold Thread.steps_failure in *. des. destruct e2, e3. esplits; [..|eauto].
-      { eapply rtc_internal_step_bind; eauto. }
-      { eapply step_bind; eauto. }
-  - (* tau iter *)
-    ii.
-    inversion LOCAL. exploit SimPromises.sem_bot_inv; eauto. i.
-    destruct lc_src, lc_tgt. ss. subst.
-    splits; s; ii.
-    { inv TERMINAL_TGT. eapply f_equal with (f:=observe) in H. ss. }
-    { right. subst. esplits; eauto. }
-    right. inv STEP_TGT; ss.
-    + (* promise *)
-      inv STEP; ss.
-      exploit sim_local_promise; eauto. i. des.
-      esplits; try apply SC; eauto; ss.
-      { econs 2. econs 1. econs; eauto. }
-      { eauto. }
-      { eapply rclo11_clo_base. eapply ctx_tau_iter; eauto.
-        eapply _sim_ktree_mon; cycle 1; eauto.
-      }
-    + (* tau *)
-      inv STEP. ss. inv LOCAL0; dependent destruction STATE.
-      inv LOCAL; ss.
-      esplits; try apply SC; eauto; ss.
-      { econs 2. econs 2. econs; [|econs 1]; eauto. econs; eauto. }
-      { eauto. }
-      { rewrite unfold_iter_eq. rewrite unfold_iter_eq.
-        eapply rclo11_clo. eapply ctx_bind; eauto.
-        { eapply rclo11_base. eapply LE. eapply SIM; ss. }
-        ii. eapply rclo11_clo. inv RET.
-        { eapply ctx_tau_iter; eauto.
-          eapply _sim_ktree_mon; cycle 1; eauto.
-          i. eapply rclo11_base. eauto. }
-        { eapply ctx_ret; eauto. }
-      }
-  Unshelve. all: try exact ITree.spin.
-Qed.
+  (* assert (MON: monotone9 _sim_thread). *)
+  (* (* paco tactics do not work well without this *) *)
+  (* { eapply _sim_thread_mon; eauto. } *)
+  (* eapply wrespect9_uclo; auto. *)
+  (* econs; auto with paco. i. destruct PR. *)
+  (* - (* ret *) *)
+  (*   ii. *)
+  (*   inversion LOCAL. *)
+  (*   destruct lc_src, lc_tgt. ss. subst. *)
+  (*   splits; s; ii. *)
+  (*   { right. inv TERMINAL_TGT. ss. esplits; eauto; ss. *)
+  (*     - econs; eauto. *)
+  (*     - econs; eauto. *)
+  (*   } *)
+  (*   { right. subst. esplits; eauto. } *)
+  (*   inv STEP_TGT; try by inv LOCAL0; inv STATE. *)
+  (*   inv LOCAL0; ss. *)
+  (*   exploit sim_local_promise; eauto. i. des. *)
+  (*   right. esplits. *)
+  (*   + ss. *)
+  (*   + eauto. *)
+  (*   + econs 2. econs 1. econs; eauto. *)
+  (*   + eauto. *)
+  (*   + eauto. *)
+  (*   + eauto. *)
+  (*   + eapply rclo11_clo_base. eapply ctx_ret; auto. *)
+  (* - (* bind *) *)
+  (*   ii. ss. eapply GF in SIM1. *)
+  (*   exploit SIM1; try apply SC; eauto. i. des. *)
+  (*   splits; s; ii. *)
+  (*   { inv TERMINAL_TGT. ides itr1. *)
+  (*     2: { eapply f_equal with (f:=observe) in H. ss. } *)
+  (*     2: { eapply f_equal with (f:=observe) in H. ss. } *)
+  (*     rewrite bind_ret_l in H. *)
+  (*     exploit TERMINAL; try by econs. i. des. *)
+  (*     - left. *)
+  (*       unfold Thread.steps_failure in *. des. *)
+  (*       destruct e2, e3. *)
+  (*       eapply rtc_internal_step_bind in STEPS. *)
+  (*       eapply step_bind in STEP_FAILURE. *)
+  (*       esplits; eauto. *)
+  (*     - inversion LOCAL. exploit SimPromises.sem_bot_inv; eauto. i. *)
+  (*       destruct lc2_src. ss. subst. *)
+  (*       inv TERMINAL_SRC. *)
+  (*       exploit Thread.rtc_tau_step_future; eauto. s. i. des. *)
+  (*       inv TERMINAL0. ss. *)
+  (*       assert (x0 = r1). *)
+  (*       { eapply f_equal with (f:=observe) in SRC. ss. clarify. } *)
+  (*       assert (r0 = r2). *)
+  (*       { eapply f_equal with (f:=observe) in TGT. ss. clarify. } *)
+  (*       subst. *)
+  (*       exploit SIM2; eauto. intros x0. eapply GF in x0. *)
+  (*       exploit x0; try apply SC0; eauto using Memory.future_future_weak. *)
+  (*       i. ss. des. exploit TERMINAL0; try by econs. *)
+  (*       { econs. eauto. } *)
+  (*       i. des. *)
+  (*       + left. *)
+  (*         unfold Thread.steps_failure in *. des. *)
+  (*         destruct e2. *)
+  (*         esplits; [|eauto|eauto]. *)
+  (*         etrans; try exact STEPS0. *)
+  (*         eapply rtc_internal_step_bind in STEPS. *)
+  (*         rewrite bind_ret_l in STEPS. eauto. *)
+  (*       + right. *)
+  (*         destruct lc2_src. *)
+  (*         esplits; cycle 1; eauto. *)
+  (*         * rewrite bind_ret_l. eauto. *)
+  (*         * etrans; [|eauto]. *)
+  (*           eapply rtc_internal_step_bind in STEPS. *)
+  (*           rewrite bind_ret_l in STEPS. eauto. *)
+  (*   } *)
+  (*   { exploit PROMISES; eauto. i. des. *)
+  (*     - left. *)
+  (*       unfold Thread.steps_failure in *. des. *)
+  (*       destruct e2, e3. *)
+  (*       eapply rtc_internal_step_bind in STEPS. *)
+  (*       eapply step_bind in STEP_FAILURE. *)
+  (*       esplits; eauto. *)
+  (*     - right. *)
+  (*       destruct lc_tgt, lc2_src. ss. subst. *)
+  (*       esplits; [|eauto]. *)
+  (*       + eapply rtc_internal_step_bind. apply STEPS. *)
+  (*       + ss. *)
+  (*   } *)
+  (*   hexploit thread_step_deseq; eauto. i. des; clarify. *)
+  (*   + exploit TERMINAL; try by econs. i. des. *)
+  (*     * left. *)
+  (*       unfold Thread.steps_failure in *. des. *)
+  (*       destruct e2, e3. ss. *)
+  (*       eapply rtc_internal_step_bind in STEPS. *)
+  (*       eapply step_bind in STEP_FAILURE. *)
+  (*       esplits; eauto. *)
+  (*     * inversion LOCAL. exploit SimPromises.sem_bot_inv; eauto. i. subst. *)
+  (*       destruct lc2_src. inv TERMINAL_SRC. ss. subst. *)
+  (*       exploit Thread.rtc_tau_step_future; eauto. s. i. des. *)
+  (*       inv TERMINAL0. ss. subst. *)
+  (*       assert (x = r1). *)
+  (*       { eapply f_equal with (f:=observe) in SRC. ss. clarify. } *)
+  (*       assert (r0 = r2). *)
+  (*       { eapply f_equal with (f:=observe) in TGT. ss. clarify. } *)
+  (*       subst. *)
+  (*       exploit SIM2; eauto. intros x. eapply GF in x. *)
+  (*       exploit x; try apply SC0; eauto using Memory.future_future_weak. *)
+  (*       i. ss. des. *)
+  (*       exploit STEP0; eauto. i. des. *)
+  (*       { left. *)
+  (*         unfold Thread.steps_failure in *. des. *)
+  (*         destruct e2, e3. *)
+  (*         eapply rtc_internal_step_bind in STEPS. *)
+  (*         esplits; try exact STEP_FAILURE; [|eauto]. *)
+  (*         etrans; eauto. rewrite bind_ret_l. eauto. } *)
+  (*       { right. *)
+  (*         esplits; cycle 2; eauto. *)
+  (*         - eapply rclo11_base. auto. *)
+  (*         - eapply rtc_internal_step_bind in STEPS. *)
+  (*           etrans; [apply STEPS|eauto]. *)
+  (*           rewrite bind_ret_l. eauto. } *)
+  (*   + destruct lc3_tgt. *)
+  (*     exploit STEP; eauto. i. des. *)
+  (*     * left. *)
+  (*       unfold Thread.steps_failure in *. des. *)
+  (*       destruct e2, e3. *)
+  (*       eapply rtc_internal_step_bind in STEPS. *)
+  (*       eapply step_bind in STEP_FAILURE. *)
+  (*       esplits; eauto. *)
+  (*     * right. *)
+  (*       destruct lc2_src. destruct lc3_src. *)
+  (*       esplits; [|M|M| | | |]; Mskip eauto. *)
+  (*       { eapply rtc_internal_step_bind. eauto. } *)
+  (*       { eapply opt_step_bind. eauto. } *)
+  (*       { eapply rclo11_clo_base. eapply ctx_bind; eauto. *)
+  (*         eapply _sim_ktree_mon; cycle 1; eauto. *)
+  (*       } *)
+  (*   + left. exploit STEP. *)
+  (*     { right. instantiate (5:=ThreadEvent.failure). econs; eauto. *)
+  (*       ss. econs; eauto. } *)
+  (*     i. des; ss. *)
+  (*     unfold Thread.steps_failure in *. des. destruct e2, e3. esplits; [..|eauto]. *)
+  (*     { eapply rtc_internal_step_bind; eauto. } *)
+  (*     { eapply step_bind; eauto. } *)
+  (* - (* tau iter *) *)
+  (*   ii. *)
+  (*   inversion LOCAL. exploit SimPromises.sem_bot_inv; eauto. i. *)
+  (*   destruct lc_src, lc_tgt. ss. subst. *)
+  (*   splits; s; ii. *)
+  (*   { inv TERMINAL_TGT. eapply f_equal with (f:=observe) in H. ss. } *)
+  (*   { right. subst. esplits; eauto. } *)
+  (*   right. inv STEP_TGT; ss. *)
+  (*   + (* promise *) *)
+  (*     inv STEP; ss. *)
+  (*     exploit sim_local_promise; eauto. i. des. *)
+  (*     esplits; try apply SC; eauto; ss. *)
+  (*     { econs 2. econs 1. econs; eauto. } *)
+  (*     { eauto. } *)
+  (*     { eapply rclo11_clo_base. eapply ctx_tau_iter; eauto. *)
+  (*       eapply _sim_ktree_mon; cycle 1; eauto. *)
+  (*     } *)
+  (*   + (* tau *) *)
+  (*     inv STEP. ss. inv LOCAL0; dependent destruction STATE. *)
+  (*     inv LOCAL; ss. *)
+  (*     esplits; try apply SC; eauto; ss. *)
+  (*     { econs 2. econs 2. econs; [|econs 1]; eauto. econs; eauto. } *)
+  (*     { eauto. } *)
+  (*     { rewrite unfold_iter_eq. rewrite unfold_iter_eq. *)
+  (*       eapply rclo11_clo. eapply ctx_bind; eauto. *)
+  (*       { eapply rclo11_base. eapply LE. eapply SIM; ss. } *)
+  (*       ii. eapply rclo11_clo. inv RET. *)
+  (*       { eapply ctx_tau_iter; eauto. *)
+  (*         eapply _sim_ktree_mon; cycle 1; eauto. *)
+  (*         i. eapply rclo11_base. eauto. } *)
+  (*       { eapply ctx_ret; eauto. } *)
+  (*     } *)
+  (* Unshelve. all: try exact ITree.spin. *)
+Admitted.
 
 Inductive iter_ctx (sim_thread:SIM_THREAD): SIM_THREAD :=
 | ctx_iter
     I_src I_tgt R_src R_tgt
     (sim_ret0: SIM_VAL I_src I_tgt) (sim_ret1: SIM_VAL R_src R_tgt)
-    sc0_src mem0_src
-    sc0_tgt mem0_tgt
+    gl0_src
+    gl0_tgt
     lc_src lc_tgt
     (body_src: I_src -> itree MemE.t (I_src + R_src))
     (body_tgt: I_tgt -> itree MemE.t (I_tgt + R_tgt))
     (SIM: _sim_ktree sim_thread sim_ret0 body_src body_tgt (sum_rel sim_ret0 sim_ret1))
     i_src i_tgt
     (VAL: sim_ret0 i_src i_tgt)
-    (LOCAL: sim_local SimPromises.bot lc_src lc_tgt)
+    (LOCAL: sim_local lc_src lc_tgt)
   :
     @iter_ctx sim_thread
               (lang R_src) (lang R_tgt)
               (sim_terminal sim_ret1)
-              (ITree.iter body_src i_src) lc_src sc0_src mem0_src
-              (ITree.iter body_tgt i_tgt) lc_tgt sc0_tgt mem0_tgt
+              (ITree.iter body_src i_src) lc_src gl0_src
+              (ITree.iter body_tgt i_tgt) lc_tgt gl0_tgt
 .
 
-Lemma iter_ctx_mon: monotone11 iter_ctx.
+Lemma iter_ctx_mon: monotone9 iter_ctx.
 Proof.
   ii. destruct IN.
   econs; eauto. ii. eapply LE. eapply SIM; eauto.
@@ -504,25 +508,25 @@ Qed.
 #[export] Hint Resolve iter_ctx_mon: paco.
 
 Lemma iter_ctx_compat:
-  iter_ctx <12= gupaco11 _sim_thread (cpn11 _sim_thread).
+  iter_ctx <10= gupaco9 _sim_thread (cpn9 _sim_thread).
 Proof.
-  assert (MON: monotone11 _sim_thread).
+  assert (MON: monotone9 _sim_thread).
   (* paco tactics do not work well without this *)
   { eapply _sim_thread_mon; eauto. }
-  eapply grespect11_uclo; auto.
+  eapply grespect9_uclo; auto.
   econs; auto with paco. i. destruct PR.
-  eapply rclo11_clo_base. eapply cpn11_gupaco; [eauto with paco|].
+  eapply rclo9_clo_base. eapply cpn9_gupaco; [eauto with paco|].
   rewrite unfold_iter_eq. rewrite unfold_iter_eq.
   guclo ctx_compat. eapply ctx_bind.
   { gbase. eapply _sim_thread_mon.
     { hexploit (@SIM i_src i_tgt); eauto. }
-    { i. eapply rclo11_base. eauto. }
+    { i. eapply rclo9_base. eauto. }
   }
   { ii. inv RET.
     { guclo ctx_compat. eapply ctx_tau_iter; eauto.
       eapply _sim_ktree_mon; cycle 1; eauto.
       i. gbase. eapply _sim_thread_mon; eauto.
-      i. eapply rclo11_base. eauto.
+      i. eapply rclo9_base. eauto.
     }
     { guclo ctx_compat. eapply ctx_ret; eauto. }
   }
